202502040951
Status: #idea
Tags:

$$\frac{10}{s(s+3)} = \frac{A}{s} + \frac{B}{s+3}$$
$$
= \frac{A(s+3) + B(s) }{s(s+3)}
$$
set numerators equal to each other

$$
10 = As + 3A + Bs = 3A + s(A+B)
$$
3A is your constant term, so set $3A = 10$, giving $A = \frac{10}{3}$ 
now, solve the rest equal to zero
$$
0 = A + B,\frac{10}{3}+B = 0, B=-\frac{10}{3}
$$
now, plug in A and B to original equation
$$
\frac{10}{s(s+3)} = \frac{10/3}{s} + \frac{-10/3}{s+3}
$$
$$ \frac{A}{s} + \frac{B}{s+\frac{1}{RC}}$$
$$ (A+B)s + \frac{A}{RC}) $$